Update arithmetic_expression.lean

ch8/arithmetic_expression.lean
@@ -6,8 +6,8 @@ inductive aexpr : Type
 
 open aexpr
 
-def sample_aexpr : aexpr :=
-plus (times (var 0) (const 7)) (times (const 2) (var 1))
+def sample_aexpr : aexpr := 
+times (plus (times (var 0) (const 7)) (times (const 2) (var 1))) (const 2)
 
 -- BEGIN
 def aeval (v : ℕ → ℕ) : aexpr → ℕ
@@ -22,9 +22,18 @@ def sample_val : ℕ → ℕ
 | _ := 0
 
 -- Try it out. You should get 47 here.
+#eval sample_aexpr
 #eval aeval sample_val sample_aexpr
 -- END
 
+def to_str : aexpr → string
+| (const n)    := to_string n
+| (var n)      := "var" ++ to_string n
+| (plus e₁ e₂)    := to_str e₁ ++ " + " ++ to_str e₂ 
+| (times e₁ e₂) := "(" ++ to_str e₁ ++ ") * " ++ "(" ++ to_str e₂ ++ ")" 
+
+instance aexpr_has_repr : has_repr aexpr := has_repr.mk (to_str)
+#eval sample_aexpr
 
 -- BEGIN
 def simp_const : aexpr → aexpr
@@ -33,39 +42,41 @@ def simp_const : aexpr → aexpr
 | e                             := e
 
 def fuse : aexpr → aexpr 
-| (times e₁ e₂) := times  (fuse e₁) (fuse e₂)
-| (plus e₁ e₂) := plus (fuse e₁) (fuse e₂)
+| (plus (const n₁) (const n₂))  := const (n₁ + n₂)
+| (times (const n₁) (const n₂)) := const (n₁ * n₂)
+| (times e₁ e₂) := simp_const (times  (fuse e₁) (fuse e₂))
+| (plus e₁ e₂) := simp_const (plus (fuse e₁) (fuse e₂))
 | e                             := simp_const e
 -- how to do this otherwise?
 
+def sample_redundant_consts : aexpr := 
+plus (const 5) (const 7)
+
+def sample_redundant_expr : aexpr :=
+
+plus (times ( plus (const 1) (const 2) ) (var 1) ) ( times (const 8) (const 3))
+
+def sample_more_redundant_expr : aexpr := 
+plus(
+  times 
+  (times (plus (const 5) (const 7)) (var 0)) (times (const 3) (const 2))
+  )
+  (plus (plus (plus (const 3) (const 5)) (const 6)) (const 10))
+
+#eval sample_redundant_consts
+#eval simp_const sample_redundant_consts -- 12
+
+#eval sample_redundant_expr
+#eval simp_const sample_redundant_expr -- does nothing
+#eval fuse sample_redundant_expr -- i think this follows specification 
+
+#eval sample_more_redundant_expr
+#eval fuse sample_more_redundant_expr
+
+
+
+
 theorem simp_const_eq (v : ℕ → ℕ) :
-  ∀ e : aexpr, aeval v (simp_const e) = aeval v e :=
-begin
-  intro e,
-  induction e with _ _ a b _ _ a b _ _,
-  { refl },
-  { refl },
-  { cases a,
-    cases b,
-    { refl },
-    { refl },
-    { refl },
-    { refl },
-    { refl },
-    { refl },
-    { refl } },
-  { cases a,
-    cases b,
-    { refl },
-    { refl },
-    { refl },
-    { refl },
-    { refl },
-    { refl },
-    { refl },
-  }
-end
-theorem simp_const_eq_faster (v : ℕ → ℕ) :
   ∀ e : aexpr, aeval v (simp_const e) = aeval v e :=
   begin
   intro e,
@@ -84,39 +95,21 @@ theorem simp_const_eq_faster (v : ℕ → ℕ) :
   repeat {rw simp_const},
   repeat {rw aeval},
   end
-
-
-
 theorem fuse_eq (v : ℕ → ℕ) :
   ∀ e : aexpr, aeval v (fuse e) = aeval v e :=
 begin
-
 intro e,
-induction e with _ _ a b _ _  a b _ _,
-{refl,},
-{refl,},
-{ cases a,
-  cases b,
-  {refl,},
-  {refl,},
-  {rw fuse, rw aeval, rw e_ih_ᾰ_1, refl,},
-  {rw fuse, rw aeval, rw e_ih_ᾰ_1, refl,},
-  {simp [fuse, aeval, simp_const, e_ih_ᾰ_1, e_ih_ᾰ],},
-  {rw fuse, rw aeval, rw e_ih_ᾰ, simp [fuse, aeval, simp_const, e_ih_ᾰ, e_ih_ᾰ_1], },
-  {rw fuse, rw aeval, rw e_ih_ᾰ, simp [fuse, aeval, simp_const, e_ih_ᾰ_1, e_ih_ᾰ], },
-},
-{ cases a,
-  cases b,
-  {refl,},
-  {refl,},
-  {rw fuse, rw aeval, rw e_ih_ᾰ_1, refl,},
-  {rw fuse, rw aeval, rw e_ih_ᾰ_1, refl,},
-  {simp [fuse, aeval, simp_const, e_ih_ᾰ_1, e_ih_ᾰ],},
-  {rw fuse, rw aeval, rw e_ih_ᾰ, simp [fuse, aeval, simp_const, e_ih_ᾰ_1, e_ih_ᾰ], },
-  {rw fuse, rw aeval, rw e_ih_ᾰ, simp [fuse, aeval, simp_const, e_ih_ᾰ_1, e_ih_ᾰ], },
-}
+induction e with h1 h2 h3 h4 h5 h6 h7 h8 h9 h10 h11 h12 h13,
+refl,
+refl,
 
+cases h3,
+cases h4,
+repeat {simp [simp_const_eq, fuse, simp_const, aeval, h6, h5]},
 
+cases h7,
+cases h8,
+repeat {simp [simp_const_eq, fuse, simp_const, aeval, h9, h10]},
 
 end
 -- END
